strengthen EssentialInterruptContinuationInvariantProperties, nix assume
 * have EssentialInterruptContinuationInvariantProperties require the
   continuation to leave the bottom bit of SP clear, in agreement with
   the special-case return path from printInterruptHandlerReturn()
   (otherwise it returns to the usermode continuation)

 * use this in a proof, so that if the handler returned with the
   original (sane) SP, then we can't have taken a FIQ from supervisor
   mode

still not entirely comfortable with this approach, but it's probably
close to the best we can do given that the control flow is all in
trusted code anyway

verified/ARMdef.s.dfy
@@ -686,14 +686,19 @@ function havocUserRegs(nondet:int, us:UserState, regs:map<ARMReg, word>): map<AR
 // To be defined/established by "application" code (i.e. komodo exception handlers)
 // XXX: for soundness, application must prove the essential properties
 
+// essential properties for the usermode continuation (must return)
 predicate EssentialContinuationInvariantProperties(s:state, r:state)
 {
     (ValidState(s) ==> ValidState(r)) && (s.ok ==> r.ok)
 }
 
+// essential properties for the interrupt-handler continuation (might not return)
 predicate EssentialInterruptContinuationInvariantProperties(s:state, r:state)
 {
     EssentialContinuationInvariantProperties(s, r) && !interrupts_enabled(r)
+    // this is needed for the special-case return in printInterruptHandlerReturn
+    // (the continuation only returns if SP & 1 == 0)
+    && (ValidState(r) && r.ok ==> evalOBool(r, OCmp(OTstEq, OSP, OConst(1))))
 }
 
 predicate {:axiom} UsermodeContinuationPrecondition(s:state)
@@ -714,7 +719,7 @@ predicate {:axiom} InterruptContinuationInvariant(s:state, r:state)
         // B1.8.3 "Link values saved on exception entry"
         // these are necessary to get MOVS PC, LR to restore the same PC
         // (this is needed here, because we don't model the PC explicitly)
-        && OperandContents(r, OLR) == TruncateWord(OperandContents(s, OLR) - 4))
+        && (ValidState(r) ==> OperandContents(r, OLR) == TruncateWord(OperandContents(s, OLR) - 4)))
 
 //-----------------------------------------------------------------------------
 // Model of page tables for userspace execution
@@ -1055,7 +1060,7 @@ function evalOBool(s:state, o:obool):bool
 predicate evalGuard(s:state, o:obool, r:state)
     requires ValidState(s) && ValidOperand(o.o1) && ValidOperand(o.o2)
 {
-    // TODO: this is where we havoc the flags for the comparison, once we model them
+    // this is where we would havoc flags for comparisons, if we modelled them
     maybeHandleInterrupt(s, r)
 }
 
